proofs/fstar/extraction/Ristretto255.Bundle.fst
@@ -1,0 +1,892 @@
+module Ristretto255.Bundle
+#set-options "--fuel 0 --ifuel 1 --z3rlimit 15"
+open FStar.Mul
+open Core_models
+
+let _ =
+  (* This module has implicit dependencies, here we make them explicit. *)
+  (* The implicit dependencies arise from typeclasses instances. *)
+  let open Curve25519_dalek.Traits in
+  let open Subtle in
+  ()
+
+type t_FieldElement = | FieldElement : t_Array u64 (mk_usize 5) -> t_FieldElement
+
+/// Edwards `d` value, equal to `-121665/121666 mod p`.
+let v_EDWARDS_D: t_FieldElement =
+  FieldElement
+  (let list =
+      [
+        mk_u64 929955233495203;
+        mk_u64 466365720129213;
+        mk_u64 1662059464998953;
+        mk_u64 2033849074728123;
+        mk_u64 1442794654840575
+      ]
+    in
+    FStar.Pervasives.assert_norm (Prims.eq2 (List.Tot.length list) 5);
+    Rust_primitives.Hax.array_of_list 5 list)
+  <:
+  t_FieldElement
+
+/// Precomputed value of one of the square roots of -1 (mod p).
+let v_SQRT_M1: t_FieldElement =
+  FieldElement
+  (let list =
+      [
+        mk_u64 1718705420411056;
+        mk_u64 234908883556509;
+        mk_u64 2233514472574048;
+        mk_u64 2117202627021982;
+        mk_u64 765476049583133
+      ]
+    in
+    FStar.Pervasives.assert_norm (Prims.eq2 (List.Tot.length list) 5);
+    Rust_primitives.Hax.array_of_list 5 list)
+  <:
+  t_FieldElement
+
+let impl_12: Core_models.Clone.t_Clone t_FieldElement =
+  { f_clone = (fun x -> x); f_clone_pre = (fun _ -> True); f_clone_post = (fun _ _ -> True) }
+
+[@@ FStar.Tactics.Typeclasses.tcinstance]
+assume
+val impl_13': Core_models.Marker.t_Copy t_FieldElement
+
+unfold
+let impl_13 = impl_13'
+
+[@@ FStar.Tactics.Typeclasses.tcinstance]
+assume
+val impl_14': Core_models.Fmt.t_Debug t_FieldElement
+
+unfold
+let impl_14 = impl_14'
+
+[@@ FStar.Tactics.Typeclasses.tcinstance]
+assume
+val impl_15': Core_models.Marker.t_StructuralPartialEq t_FieldElement
+
+unfold
+let impl_15 = impl_15'
+
+[@@ FStar.Tactics.Typeclasses.tcinstance]
+assume
+val impl_16': Core_models.Cmp.t_PartialEq t_FieldElement t_FieldElement
+
+unfold
+let impl_16 = impl_16'
+
+[@@ FStar.Tactics.Typeclasses.tcinstance]
+assume
+val impl_17': Core_models.Cmp.t_Eq t_FieldElement
+
+unfold
+let impl_17 = impl_17'
+
+[@@ FStar.Tactics.Typeclasses.tcinstance]
+let impl: Curve25519_dalek.Traits.t_Identity t_FieldElement =
+  {
+    f_identity_pre = (fun (_: Prims.unit) -> true);
+    f_identity_post = (fun (_: Prims.unit) (out: t_FieldElement) -> true);
+    f_identity
+    =
+    fun (_: Prims.unit) ->
+      FieldElement (Rust_primitives.Hax.repeat (mk_u64 0) (mk_usize 5)) <: t_FieldElement
+  }
+
+[@@ FStar.Tactics.Typeclasses.tcinstance]
+let impl_2: Core_models.Ops.Arith.t_Add t_FieldElement t_FieldElement =
+  {
+    f_Output = t_FieldElement;
+    f_add_pre = (fun (self: t_FieldElement) (rhs: t_FieldElement) -> true);
+    f_add_post = (fun (self: t_FieldElement) (rhs: t_FieldElement) (out1: t_FieldElement) -> true);
+    f_add
+    =
+    fun (self: t_FieldElement) (rhs: t_FieldElement) ->
+      let out:t_Array u64 (mk_usize 5) = Rust_primitives.Hax.repeat (mk_u64 0) (mk_usize 5) in
+      let out:t_Array u64 (mk_usize 5) =
+        Libcrux_hacl_rs.Bignum25519_51_.fadd out (self._0 <: t_Slice u64) (rhs._0 <: t_Slice u64)
+      in
+      FieldElement out <: t_FieldElement
+  }
+
+[@@ FStar.Tactics.Typeclasses.tcinstance]
+let impl_3: Core_models.Ops.Arith.t_Sub t_FieldElement t_FieldElement =
+  {
+    f_Output = t_FieldElement;
+    f_sub_pre = (fun (self: t_FieldElement) (rhs: t_FieldElement) -> true);
+    f_sub_post = (fun (self: t_FieldElement) (rhs: t_FieldElement) (out1: t_FieldElement) -> true);
+    f_sub
+    =
+    fun (self: t_FieldElement) (rhs: t_FieldElement) ->
+      let out:t_Array u64 (mk_usize 5) = Rust_primitives.Hax.repeat (mk_u64 0) (mk_usize 5) in
+      let out:t_Array u64 (mk_usize 5) =
+        Libcrux_hacl_rs.Bignum25519_51_.fsub out (self._0 <: t_Slice u64) (rhs._0 <: t_Slice u64)
+      in
+      FieldElement out <: t_FieldElement
+  }
+
+[@@ FStar.Tactics.Typeclasses.tcinstance]
+let impl_4: Core_models.Ops.Arith.t_Mul t_FieldElement u64 =
+  {
+    f_Output = t_FieldElement;
+    f_mul_pre = (fun (self: t_FieldElement) (rhs: u64) -> true);
+    f_mul_post = (fun (self: t_FieldElement) (rhs: u64) (out1: t_FieldElement) -> true);
+    f_mul
+    =
+    fun (self: t_FieldElement) (rhs: u64) ->
+      let out:t_Array u64 (mk_usize 5) = Rust_primitives.Hax.repeat (mk_u64 0) (mk_usize 5) in
+      let out:t_Array u64 (mk_usize 5) =
+        Libcrux_hacl_rs.Bignum25519_51_.fmul1 out (self._0 <: t_Slice u64) rhs
+      in
+      FieldElement out <: t_FieldElement
+  }
+
+[@@ FStar.Tactics.Typeclasses.tcinstance]
+let impl_5: Core_models.Ops.Arith.t_Mul t_FieldElement t_FieldElement =
+  {
+    f_Output = t_FieldElement;
+    f_mul_pre = (fun (self: t_FieldElement) (rhs: t_FieldElement) -> true);
+    f_mul_post = (fun (self: t_FieldElement) (rhs: t_FieldElement) (out1: t_FieldElement) -> true);
+    f_mul
+    =
+    fun (self: t_FieldElement) (rhs: t_FieldElement) ->
+      let out:t_Array u64 (mk_usize 5) = Rust_primitives.Hax.repeat (mk_u64 0) (mk_usize 5) in
+      let (tmp: t_Array u128 (mk_usize 10)):t_Array u128 (mk_usize 10) =
+        Rust_primitives.Hax.repeat (Libcrux_hacl_rs.Fstar.Uint128.uint64_to_uint128 (mk_u64 0)
+            <:
+            u128)
+          (mk_usize 10)
+      in
+      let out:t_Array u64 (mk_usize 5) =
+        Libcrux_hacl_rs.Bignum25519_51_.fmul out
+          (self._0 <: t_Slice u64)
+          (rhs._0 <: t_Slice u64)
+          (tmp <: t_Slice u128)
+      in
+      FieldElement out <: t_FieldElement
+  }
+
+let impl_6__ONE: t_FieldElement =
+  FieldElement
+  (let list = [mk_u64 1; mk_u64 0; mk_u64 0; mk_u64 0; mk_u64 0] in
+    FStar.Pervasives.assert_norm (Prims.eq2 (List.Tot.length list) 5);
+    Rust_primitives.Hax.array_of_list 5 list)
+  <:
+  t_FieldElement
+
+/// Serialize this field element to canonical 32-byte encoding.
+/// Adapted from the `curve25519-dalek` crate.
+let impl_6__to_bytes (self: t_FieldElement) : t_Array u8 (mk_usize 32) =
+  let low_51_bit_mask:u64 = (mk_u64 1 <<! mk_i32 51 <: u64) -! mk_u64 1 in
+  let limbs:t_Array u64 (mk_usize 5) = self._0 in
+  let limbs:t_Array u64 (mk_usize 5) =
+    Rust_primitives.Hax.Monomorphized_update_at.update_at_usize limbs
+      (mk_usize 1)
+      ((limbs.[ mk_usize 1 ] <: u64) +! ((limbs.[ mk_usize 0 ] <: u64) >>! mk_i32 51 <: u64) <: u64)
+  in
+  let limbs:t_Array u64 (mk_usize 5) =
+    Rust_primitives.Hax.Monomorphized_update_at.update_at_usize limbs
+      (mk_usize 0)
+      ((limbs.[ mk_usize 0 ] <: u64) &. low_51_bit_mask <: u64)
+  in
+  let limbs:t_Array u64 (mk_usize 5) =
+    Rust_primitives.Hax.Monomorphized_update_at.update_at_usize limbs
+      (mk_usize 2)
+      ((limbs.[ mk_usize 2 ] <: u64) +! ((limbs.[ mk_usize 1 ] <: u64) >>! mk_i32 51 <: u64) <: u64)
+  in
+  let limbs:t_Array u64 (mk_usize 5) =
+    Rust_primitives.Hax.Monomorphized_update_at.update_at_usize limbs
+      (mk_usize 1)
+      ((limbs.[ mk_usize 1 ] <: u64) &. low_51_bit_mask <: u64)
+  in
+  let limbs:t_Array u64 (mk_usize 5) =
+    Rust_primitives.Hax.Monomorphized_update_at.update_at_usize limbs
+      (mk_usize 3)
+      ((limbs.[ mk_usize 3 ] <: u64) +! ((limbs.[ mk_usize 2 ] <: u64) >>! mk_i32 51 <: u64) <: u64)
+  in
+  let limbs:t_Array u64 (mk_usize 5) =
+    Rust_primitives.Hax.Monomorphized_update_at.update_at_usize limbs
+      (mk_usize 2)
+      ((limbs.[ mk_usize 2 ] <: u64) &. low_51_bit_mask <: u64)
+  in
+  let limbs:t_Array u64 (mk_usize 5) =
+    Rust_primitives.Hax.Monomorphized_update_at.update_at_usize limbs
+      (mk_usize 4)
+      ((limbs.[ mk_usize 4 ] <: u64) +! ((limbs.[ mk_usize 3 ] <: u64) >>! mk_i32 51 <: u64) <: u64)
+  in
+  let limbs:t_Array u64 (mk_usize 5) =
+    Rust_primitives.Hax.Monomorphized_update_at.update_at_usize limbs
+      (mk_usize 3)
+      ((limbs.[ mk_usize 3 ] <: u64) &. low_51_bit_mask <: u64)
+  in
+  let limbs:t_Array u64 (mk_usize 5) =
+    Rust_primitives.Hax.Monomorphized_update_at.update_at_usize limbs
+      (mk_usize 0)
+      ((limbs.[ mk_usize 0 ] <: u64) +!
+        (((limbs.[ mk_usize 4 ] <: u64) >>! mk_i32 51 <: u64) *! mk_u64 19 <: u64)
+        <:
+        u64)
+  in
+  let limbs:t_Array u64 (mk_usize 5) =
+    Rust_primitives.Hax.Monomorphized_update_at.update_at_usize limbs
+      (mk_usize 4)
+      ((limbs.[ mk_usize 4 ] <: u64) &. low_51_bit_mask <: u64)
+  in
+  let limbs:t_Array u64 (mk_usize 5) =
+    Rust_primitives.Hax.Monomorphized_update_at.update_at_usize limbs
+      (mk_usize 1)
+      ((limbs.[ mk_usize 1 ] <: u64) +! ((limbs.[ mk_usize 0 ] <: u64) >>! mk_i32 51 <: u64) <: u64)
+  in
+  let limbs:t_Array u64 (mk_usize 5) =
+    Rust_primitives.Hax.Monomorphized_update_at.update_at_usize limbs
+      (mk_usize 0)
+      ((limbs.[ mk_usize 0 ] <: u64) &. low_51_bit_mask <: u64)
+  in
+  let q:u64 = ((limbs.[ mk_usize 0 ] <: u64) +! mk_u64 19 <: u64) >>! mk_i32 51 in
+  let q:u64 = ((limbs.[ mk_usize 1 ] <: u64) +! q <: u64) >>! mk_i32 51 in
+  let q:u64 = ((limbs.[ mk_usize 2 ] <: u64) +! q <: u64) >>! mk_i32 51 in
+  let q:u64 = ((limbs.[ mk_usize 3 ] <: u64) +! q <: u64) >>! mk_i32 51 in
+  let q:u64 = ((limbs.[ mk_usize 4 ] <: u64) +! q <: u64) >>! mk_i32 51 in
+  let limbs:t_Array u64 (mk_usize 5) =
+    Rust_primitives.Hax.Monomorphized_update_at.update_at_usize limbs
+      (mk_usize 0)
+      ((limbs.[ mk_usize 0 ] <: u64) +! (mk_u64 19 *! q <: u64) <: u64)
+  in
+  let limbs:t_Array u64 (mk_usize 5) =
+    Rust_primitives.Hax.Monomorphized_update_at.update_at_usize limbs
+      (mk_usize 1)
+      ((limbs.[ mk_usize 1 ] <: u64) +! ((limbs.[ mk_usize 0 ] <: u64) >>! mk_i32 51 <: u64) <: u64)
+  in
+  let limbs:t_Array u64 (mk_usize 5) =
+    Rust_primitives.Hax.Monomorphized_update_at.update_at_usize limbs
+      (mk_usize 0)
+      ((limbs.[ mk_usize 0 ] <: u64) &. low_51_bit_mask <: u64)
+  in
+  let limbs:t_Array u64 (mk_usize 5) =
+    Rust_primitives.Hax.Monomorphized_update_at.update_at_usize limbs
+      (mk_usize 2)
+      ((limbs.[ mk_usize 2 ] <: u64) +! ((limbs.[ mk_usize 1 ] <: u64) >>! mk_i32 51 <: u64) <: u64)
+  in
+  let limbs:t_Array u64 (mk_usize 5) =
+    Rust_primitives.Hax.Monomorphized_update_at.update_at_usize limbs
+      (mk_usize 1)
+      ((limbs.[ mk_usize 1 ] <: u64) &. low_51_bit_mask <: u64)
+  in
+  let limbs:t_Array u64 (mk_usize 5) =
+    Rust_primitives.Hax.Monomorphized_update_at.update_at_usize limbs
+      (mk_usize 3)
+      ((limbs.[ mk_usize 3 ] <: u64) +! ((limbs.[ mk_usize 2 ] <: u64) >>! mk_i32 51 <: u64) <: u64)
+  in
+  let limbs:t_Array u64 (mk_usize 5) =
+    Rust_primitives.Hax.Monomorphized_update_at.update_at_usize limbs
+      (mk_usize 2)
+      ((limbs.[ mk_usize 2 ] <: u64) &. low_51_bit_mask <: u64)
+  in
+  let limbs:t_Array u64 (mk_usize 5) =
+    Rust_primitives.Hax.Monomorphized_update_at.update_at_usize limbs
+      (mk_usize 4)
+      ((limbs.[ mk_usize 4 ] <: u64) +! ((limbs.[ mk_usize 3 ] <: u64) >>! mk_i32 51 <: u64) <: u64)
+  in
+  let limbs:t_Array u64 (mk_usize 5) =
+    Rust_primitives.Hax.Monomorphized_update_at.update_at_usize limbs
+      (mk_usize 3)
+      ((limbs.[ mk_usize 3 ] <: u64) &. low_51_bit_mask <: u64)
+  in
+  let limbs:t_Array u64 (mk_usize 5) =
+    Rust_primitives.Hax.Monomorphized_update_at.update_at_usize limbs
+      (mk_usize 4)
+      ((limbs.[ mk_usize 4 ] <: u64) &. low_51_bit_mask <: u64)
+  in
+  let s:t_Array u8 (mk_usize 32) = Rust_primitives.Hax.repeat (mk_u8 0) (mk_usize 32) in
+  let s:t_Array u8 (mk_usize 32) =
+    Rust_primitives.Hax.Monomorphized_update_at.update_at_usize s
+      (mk_usize 0)
+      (cast (limbs.[ mk_usize 0 ] <: u64) <: u8)
+  in
+  let s:t_Array u8 (mk_usize 32) =
+    Rust_primitives.Hax.Monomorphized_update_at.update_at_usize s
+      (mk_usize 1)
+      (cast ((limbs.[ mk_usize 0 ] <: u64) >>! mk_i32 8 <: u64) <: u8)
+  in
+  let s:t_Array u8 (mk_usize 32) =
+    Rust_primitives.Hax.Monomorphized_update_at.update_at_usize s
+      (mk_usize 2)
+      (cast ((limbs.[ mk_usize 0 ] <: u64) >>! mk_i32 16 <: u64) <: u8)
+  in
+  let s:t_Array u8 (mk_usize 32) =
+    Rust_primitives.Hax.Monomorphized_update_at.update_at_usize s
+      (mk_usize 3)
+      (cast ((limbs.[ mk_usize 0 ] <: u64) >>! mk_i32 24 <: u64) <: u8)
+  in
+  let s:t_Array u8 (mk_usize 32) =
+    Rust_primitives.Hax.Monomorphized_update_at.update_at_usize s
+      (mk_usize 4)
+      (cast ((limbs.[ mk_usize 0 ] <: u64) >>! mk_i32 32 <: u64) <: u8)
+  in
+  let s:t_Array u8 (mk_usize 32) =
+    Rust_primitives.Hax.Monomorphized_update_at.update_at_usize s
+      (mk_usize 5)
+      (cast ((limbs.[ mk_usize 0 ] <: u64) >>! mk_i32 40 <: u64) <: u8)
+  in
+  let s:t_Array u8 (mk_usize 32) =
+    Rust_primitives.Hax.Monomorphized_update_at.update_at_usize s
+      (mk_usize 6)
+      (cast (((limbs.[ mk_usize 0 ] <: u64) >>! mk_i32 48 <: u64) |.
+            ((limbs.[ mk_usize 1 ] <: u64) <<! mk_i32 3 <: u64)
+            <:
+            u64)
+        <:
+        u8)
+  in
+  let s:t_Array u8 (mk_usize 32) =
+    Rust_primitives.Hax.Monomorphized_update_at.update_at_usize s
+      (mk_usize 7)
+      (cast ((limbs.[ mk_usize 1 ] <: u64) >>! mk_i32 5 <: u64) <: u8)
+  in
+  let s:t_Array u8 (mk_usize 32) =
+    Rust_primitives.Hax.Monomorphized_update_at.update_at_usize s
+      (mk_usize 8)
+      (cast ((limbs.[ mk_usize 1 ] <: u64) >>! mk_i32 13 <: u64) <: u8)
+  in
+  let s:t_Array u8 (mk_usize 32) =
+    Rust_primitives.Hax.Monomorphized_update_at.update_at_usize s
+      (mk_usize 9)
+      (cast ((limbs.[ mk_usize 1 ] <: u64) >>! mk_i32 21 <: u64) <: u8)
+  in
+  let s:t_Array u8 (mk_usize 32) =
+    Rust_primitives.Hax.Monomorphized_update_at.update_at_usize s
+      (mk_usize 10)
+      (cast ((limbs.[ mk_usize 1 ] <: u64) >>! mk_i32 29 <: u64) <: u8)
+  in
+  let s:t_Array u8 (mk_usize 32) =
+    Rust_primitives.Hax.Monomorphized_update_at.update_at_usize s
+      (mk_usize 11)
+      (cast ((limbs.[ mk_usize 1 ] <: u64) >>! mk_i32 37 <: u64) <: u8)
+  in
+  let s:t_Array u8 (mk_usize 32) =
+    Rust_primitives.Hax.Monomorphized_update_at.update_at_usize s
+      (mk_usize 12)
+      (cast (((limbs.[ mk_usize 1 ] <: u64) >>! mk_i32 45 <: u64) |.
+            ((limbs.[ mk_usize 2 ] <: u64) <<! mk_i32 6 <: u64)
+            <:
+            u64)
+        <:
+        u8)
+  in
+  let s:t_Array u8 (mk_usize 32) =
+    Rust_primitives.Hax.Monomorphized_update_at.update_at_usize s
+      (mk_usize 13)
+      (cast ((limbs.[ mk_usize 2 ] <: u64) >>! mk_i32 2 <: u64) <: u8)
+  in
+  let s:t_Array u8 (mk_usize 32) =
+    Rust_primitives.Hax.Monomorphized_update_at.update_at_usize s
+      (mk_usize 14)
+      (cast ((limbs.[ mk_usize 2 ] <: u64) >>! mk_i32 10 <: u64) <: u8)
+  in
+  let s:t_Array u8 (mk_usize 32) =
+    Rust_primitives.Hax.Monomorphized_update_at.update_at_usize s
+      (mk_usize 15)
+      (cast ((limbs.[ mk_usize 2 ] <: u64) >>! mk_i32 18 <: u64) <: u8)
+  in
+  let s:t_Array u8 (mk_usize 32) =
+    Rust_primitives.Hax.Monomorphized_update_at.update_at_usize s
+      (mk_usize 16)
+      (cast ((limbs.[ mk_usize 2 ] <: u64) >>! mk_i32 26 <: u64) <: u8)
+  in
+  let s:t_Array u8 (mk_usize 32) =
+    Rust_primitives.Hax.Monomorphized_update_at.update_at_usize s
+      (mk_usize 17)
+      (cast ((limbs.[ mk_usize 2 ] <: u64) >>! mk_i32 34 <: u64) <: u8)
+  in
+  let s:t_Array u8 (mk_usize 32) =
+    Rust_primitives.Hax.Monomorphized_update_at.update_at_usize s
+      (mk_usize 18)
+      (cast ((limbs.[ mk_usize 2 ] <: u64) >>! mk_i32 42 <: u64) <: u8)
+  in
+  let s:t_Array u8 (mk_usize 32) =
+    Rust_primitives.Hax.Monomorphized_update_at.update_at_usize s
+      (mk_usize 19)
+      (cast (((limbs.[ mk_usize 2 ] <: u64) >>! mk_i32 50 <: u64) |.
+            ((limbs.[ mk_usize 3 ] <: u64) <<! mk_i32 1 <: u64)
+            <:
+            u64)
+        <:
+        u8)
+  in
+  let s:t_Array u8 (mk_usize 32) =
+    Rust_primitives.Hax.Monomorphized_update_at.update_at_usize s
+      (mk_usize 20)
+      (cast ((limbs.[ mk_usize 3 ] <: u64) >>! mk_i32 7 <: u64) <: u8)
+  in
+  let s:t_Array u8 (mk_usize 32) =
+    Rust_primitives.Hax.Monomorphized_update_at.update_at_usize s
+      (mk_usize 21)
+      (cast ((limbs.[ mk_usize 3 ] <: u64) >>! mk_i32 15 <: u64) <: u8)
+  in
+  let s:t_Array u8 (mk_usize 32) =
+    Rust_primitives.Hax.Monomorphized_update_at.update_at_usize s
+      (mk_usize 22)
+      (cast ((limbs.[ mk_usize 3 ] <: u64) >>! mk_i32 23 <: u64) <: u8)
+  in
+  let s:t_Array u8 (mk_usize 32) =
+    Rust_primitives.Hax.Monomorphized_update_at.update_at_usize s
+      (mk_usize 23)
+      (cast ((limbs.[ mk_usize 3 ] <: u64) >>! mk_i32 31 <: u64) <: u8)
+  in
+  let s:t_Array u8 (mk_usize 32) =
+    Rust_primitives.Hax.Monomorphized_update_at.update_at_usize s
+      (mk_usize 24)
+      (cast ((limbs.[ mk_usize 3 ] <: u64) >>! mk_i32 39 <: u64) <: u8)
+  in
+  let s:t_Array u8 (mk_usize 32) =
+    Rust_primitives.Hax.Monomorphized_update_at.update_at_usize s
+      (mk_usize 25)
+      (cast (((limbs.[ mk_usize 3 ] <: u64) >>! mk_i32 47 <: u64) |.
+            ((limbs.[ mk_usize 4 ] <: u64) <<! mk_i32 4 <: u64)
+            <:
+            u64)
+        <:
+        u8)
+  in
+  let s:t_Array u8 (mk_usize 32) =
+    Rust_primitives.Hax.Monomorphized_update_at.update_at_usize s
+      (mk_usize 26)
+      (cast ((limbs.[ mk_usize 4 ] <: u64) >>! mk_i32 4 <: u64) <: u8)
+  in
+  let s:t_Array u8 (mk_usize 32) =
+    Rust_primitives.Hax.Monomorphized_update_at.update_at_usize s
+      (mk_usize 27)
+      (cast ((limbs.[ mk_usize 4 ] <: u64) >>! mk_i32 12 <: u64) <: u8)
+  in
+  let s:t_Array u8 (mk_usize 32) =
+    Rust_primitives.Hax.Monomorphized_update_at.update_at_usize s
+      (mk_usize 28)
+      (cast ((limbs.[ mk_usize 4 ] <: u64) >>! mk_i32 20 <: u64) <: u8)
+  in
+  let s:t_Array u8 (mk_usize 32) =
+    Rust_primitives.Hax.Monomorphized_update_at.update_at_usize s
+      (mk_usize 29)
+      (cast ((limbs.[ mk_usize 4 ] <: u64) >>! mk_i32 28 <: u64) <: u8)
+  in
+  let s:t_Array u8 (mk_usize 32) =
+    Rust_primitives.Hax.Monomorphized_update_at.update_at_usize s
+      (mk_usize 30)
+      (cast ((limbs.[ mk_usize 4 ] <: u64) >>! mk_i32 36 <: u64) <: u8)
+  in
+  let s:t_Array u8 (mk_usize 32) =
+    Rust_primitives.Hax.Monomorphized_update_at.update_at_usize s
+      (mk_usize 31)
+      (cast ((limbs.[ mk_usize 4 ] <: u64) >>! mk_i32 44 <: u64) <: u8)
+  in
+  let _:Prims.unit =
+    if true
+    then
+      let _:Prims.unit =
+        Hax_lib.v_assert (((s.[ mk_usize 31 ] <: u8) &. mk_u8 128 <: u8) =. mk_u8 0 <: bool)
+      in
+      ()
+  in
+  s
+
+[@@ FStar.Tactics.Typeclasses.tcinstance]
+let impl_1: Subtle.t_ConstantTimeEq t_FieldElement =
+  {
+    f_ct_eq_pre = (fun (self: t_FieldElement) (other: t_FieldElement) -> true);
+    f_ct_eq_post
+    =
+    (fun (self: t_FieldElement) (other: t_FieldElement) (out: Subtle.t_Choice) -> true);
+    f_ct_eq
+    =
+    fun (self: t_FieldElement) (other: t_FieldElement) ->
+      Subtle.f_ct_eq #(t_Slice u8)
+        #FStar.Tactics.Typeclasses.solve
+        (impl_6__to_bytes self <: t_Slice u8)
+        (impl_6__to_bytes other <: t_Slice u8)
+  }
+
+let impl_6__square (self: t_FieldElement) : t_FieldElement =
+  let (out: t_Array u64 (mk_usize 5)):t_Array u64 (mk_usize 5) =
+    Rust_primitives.Hax.repeat (mk_u64 0) (mk_usize 5)
+  in
+  let (tmp: t_Array u128 (mk_usize 10)):t_Array u128 (mk_usize 10) =
+    Rust_primitives.Hax.repeat (Libcrux_hacl_rs.Fstar.Uint128.uint64_to_uint128 (mk_u64 0) <: u128)
+      (mk_usize 10)
+  in
+  let out:t_Array u64 (mk_usize 5) =
+    Libcrux_hacl_rs.Bignum25519_51_.fsqr out (self._0 <: t_Slice u64) (tmp <: t_Slice u128)
+  in
+  FieldElement out <: t_FieldElement
+
+let impl_6__is_negative (self: t_FieldElement) : Subtle.t_Choice =
+  let bytes:t_Array u8 (mk_usize 32) = impl_6__to_bytes self in
+  Core_models.Convert.f_into #u8
+    #Subtle.t_Choice
+    #FStar.Tactics.Typeclasses.solve
+    ((bytes.[ mk_usize 0 ] <: u8) &. mk_u8 1 <: u8)
+
+let impl_6__is_zero (self: t_FieldElement) : Subtle.t_Choice =
+  let zero:t_Array u8 (mk_usize 32) = Rust_primitives.Hax.repeat (mk_u8 0) (mk_usize 32) in
+  let bytes:t_Array u8 (mk_usize 32) = impl_6__to_bytes self in
+  Subtle.f_ct_eq #(t_Slice u8)
+    #FStar.Tactics.Typeclasses.solve
+    (bytes <: t_Slice u8)
+    (zero <: t_Slice u8)
+
+let impl_6__conditional_negate (self: t_FieldElement) (choice: Subtle.t_Choice) : t_FieldElement =
+  let neg:t_FieldElement =
+    Core_models.Ops.Arith.f_sub #t_FieldElement
+      #t_FieldElement
+      #FStar.Tactics.Typeclasses.solve
+      (Curve25519_dalek.Traits.f_identity #t_FieldElement #FStar.Tactics.Typeclasses.solve ()
+        <:
+        t_FieldElement)
+      self
+  in
+  let mask:u64 =
+    Core_models.Num.impl_u64__wrapping_sub (mk_u64 0)
+      (cast (Subtle.impl_Choice__unwrap_u8 choice <: u8) <: u64)
+  in
+  let self:t_FieldElement =
+    Rust_primitives.Hax.Folds.fold_range (mk_usize 0)
+      (mk_usize 5)
+      (fun self temp_1_ ->
+          let self:t_FieldElement = self in
+          let _:usize = temp_1_ in
+          true)
+      self
+      (fun self i ->
+          let self:t_FieldElement = self in
+          let i:usize = i in
+          {
+            self with
+            _0
+            =
+            Rust_primitives.Hax.Monomorphized_update_at.update_at_usize self._0
+              i
+              ((self._0.[ i ] <: u64) ^.
+                (mask &. ((self._0.[ i ] <: u64) ^. (neg._0.[ i ] <: u64) <: u64) <: u64)
+                <:
+                u64)
+            <:
+            t_Array u64 (mk_usize 5)
+          }
+          <:
+          t_FieldElement)
+  in
+  self
+
+let impl_6__conditional_assign (self other: t_FieldElement) (choice: Subtle.t_Choice)
+    : t_FieldElement =
+  let mask:u64 =
+    Core_models.Num.impl_u64__wrapping_sub (mk_u64 0)
+      (cast (Subtle.impl_Choice__unwrap_u8 choice <: u8) <: u64)
+  in
+  let self:t_FieldElement =
+    Rust_primitives.Hax.Folds.fold_range (mk_usize 0)
+      (mk_usize 5)
+      (fun self temp_1_ ->
+          let self:t_FieldElement = self in
+          let _:usize = temp_1_ in
+          true)
+      self
+      (fun self i ->
+          let self:t_FieldElement = self in
+          let i:usize = i in
+          {
+            self with
+            _0
+            =
+            Rust_primitives.Hax.Monomorphized_update_at.update_at_usize self._0
+              i
+              ((self._0.[ i ] <: u64) ^.
+                (mask &. ((self._0.[ i ] <: u64) ^. (other._0.[ i ] <: u64) <: u64) <: u64)
+                <:
+                u64)
+            <:
+            t_Array u64 (mk_usize 5)
+          }
+          <:
+          t_FieldElement)
+  in
+  self
+
+let impl_6__from_bytes__load8_at (input: t_Array u8 (mk_usize 32)) (i: usize) : u64 =
+  (((((((cast (input.[ i ] <: u8) <: u64) |.
+              ((cast (input.[ i +! mk_usize 1 <: usize ] <: u8) <: u64) <<! mk_i32 8 <: u64)
+              <:
+              u64) |.
+            ((cast (input.[ i +! mk_usize 2 <: usize ] <: u8) <: u64) <<! mk_i32 16 <: u64)
+            <:
+            u64) |.
+          ((cast (input.[ i +! mk_usize 3 <: usize ] <: u8) <: u64) <<! mk_i32 24 <: u64)
+          <:
+          u64) |.
+        ((cast (input.[ i +! mk_usize 4 <: usize ] <: u8) <: u64) <<! mk_i32 32 <: u64)
+        <:
+        u64) |.
+      ((cast (input.[ i +! mk_usize 5 <: usize ] <: u8) <: u64) <<! mk_i32 40 <: u64)
+      <:
+      u64) |.
+    ((cast (input.[ i +! mk_usize 6 <: usize ] <: u8) <: u64) <<! mk_i32 48 <: u64)
+    <:
+    u64) |.
+  ((cast (input.[ i +! mk_usize 7 <: usize ] <: u8) <: u64) <<! mk_i32 56 <: u64)
+
+/// Load a field element from the low 255 bits of a 32-byte input.
+/// This is intentionally non-canonical: it masks the top bit and does not
+/// reject inputs >= p.
+/// Adapted from the `curve25519-dalek` crate.
+let impl_6__from_bytes (bytes: t_Array u8 (mk_usize 32)) : t_FieldElement =
+  let low_51_bit_mask:u64 = (mk_u64 1 <<! mk_i32 51 <: u64) -! mk_u64 1 in
+  FieldElement
+  (let list =
+      [
+        (impl_6__from_bytes__load8_at bytes (mk_usize 0) <: u64) &. low_51_bit_mask;
+        ((impl_6__from_bytes__load8_at bytes (mk_usize 6) <: u64) >>! mk_i32 3 <: u64) &.
+        low_51_bit_mask;
+        ((impl_6__from_bytes__load8_at bytes (mk_usize 12) <: u64) >>! mk_i32 6 <: u64) &.
+        low_51_bit_mask;
+        ((impl_6__from_bytes__load8_at bytes (mk_usize 19) <: u64) >>! mk_i32 1 <: u64) &.
+        low_51_bit_mask;
+        ((impl_6__from_bytes__load8_at bytes (mk_usize 24) <: u64) >>! mk_i32 12 <: u64) &.
+        low_51_bit_mask
+      ]
+    in
+    FStar.Pervasives.assert_norm (Prims.eq2 (List.Tot.length list) 5);
+    Rust_primitives.Hax.array_of_list 5 list)
+  <:
+  t_FieldElement
+
+[@@ FStar.Tactics.Typeclasses.tcinstance]
+let impl_7: Core_models.Ops.Arith.t_Add t_FieldElement t_FieldElement =
+  {
+    f_Output = t_FieldElement;
+    f_add_pre = (fun (self: t_FieldElement) (rhs: t_FieldElement) -> true);
+    f_add_post = (fun (self: t_FieldElement) (rhs: t_FieldElement) (out: t_FieldElement) -> true);
+    f_add
+    =
+    fun (self: t_FieldElement) (rhs: t_FieldElement) ->
+      Core_models.Ops.Arith.f_add #t_FieldElement
+        #t_FieldElement
+        #FStar.Tactics.Typeclasses.solve
+        self
+        rhs
+  }
+
+[@@ FStar.Tactics.Typeclasses.tcinstance]
+let impl_8: Core_models.Ops.Arith.t_Sub t_FieldElement t_FieldElement =
+  {
+    f_Output = t_FieldElement;
+    f_sub_pre = (fun (self: t_FieldElement) (rhs: t_FieldElement) -> true);
+    f_sub_post = (fun (self: t_FieldElement) (rhs: t_FieldElement) (out: t_FieldElement) -> true);
+    f_sub
+    =
+    fun (self: t_FieldElement) (rhs: t_FieldElement) ->
+      Core_models.Ops.Arith.f_sub #t_FieldElement
+        #t_FieldElement
+        #FStar.Tactics.Typeclasses.solve
+        self
+        rhs
+  }
+
+[@@ FStar.Tactics.Typeclasses.tcinstance]
+let impl_9: Core_models.Ops.Arith.t_Mul t_FieldElement t_FieldElement =
+  {
+    f_Output = t_FieldElement;
+    f_mul_pre = (fun (self: t_FieldElement) (rhs: t_FieldElement) -> true);
+    f_mul_post = (fun (self: t_FieldElement) (rhs: t_FieldElement) (out: t_FieldElement) -> true);
+    f_mul
+    =
+    fun (self: t_FieldElement) (rhs: t_FieldElement) ->
+      Core_models.Ops.Arith.f_mul #t_FieldElement
+        #t_FieldElement
+        #FStar.Tactics.Typeclasses.solve
+        self
+        rhs
+  }
+
+/// Raise this field element to the power (p-5)/8 = 2^252 - 3.
+let impl_6__pow_p58 (self: t_FieldElement) : t_FieldElement =
+  let acc:t_FieldElement = impl_6__ONE in
+  let acc:t_FieldElement =
+    Core_models.Iter.Traits.Iterator.f_fold (Core_models.Iter.Traits.Collect.f_into_iter #(Core_models.Iter.Adapters.Rev.t_Rev
+            (Core_models.Ops.Range.t_Range i32))
+          #FStar.Tactics.Typeclasses.solve
+          (Core_models.Iter.Traits.Iterator.f_rev #(Core_models.Ops.Range.t_Range i32)
+              #FStar.Tactics.Typeclasses.solve
+              ({
+                  Core_models.Ops.Range.f_start = mk_i32 0;
+                  Core_models.Ops.Range.f_end = mk_i32 252
+                }
+                <:
+                Core_models.Ops.Range.t_Range i32)
+            <:
+            Core_models.Iter.Adapters.Rev.t_Rev (Core_models.Ops.Range.t_Range i32))
+        <:
+        Core_models.Iter.Adapters.Rev.t_Rev (Core_models.Ops.Range.t_Range i32))
+      acc
+      (fun acc i ->
+          let acc:t_FieldElement = acc in
+          let i:i32 = i in
+          let acc:t_FieldElement = impl_6__square acc in
+          if i <>. mk_i32 1
+          then
+            let acc:t_FieldElement =
+              Core_models.Ops.Arith.f_mul #t_FieldElement
+                #t_FieldElement
+                #FStar.Tactics.Typeclasses.solve
+                acc
+                self
+            in
+            acc
+          else acc)
+  in
+  acc
+
+[@@ FStar.Tactics.Typeclasses.tcinstance]
+let impl_10: Core_models.Ops.Arith.t_Neg t_FieldElement =
+  {
+    f_Output = t_FieldElement;
+    f_neg_pre = (fun (self: t_FieldElement) -> true);
+    f_neg_post = (fun (self: t_FieldElement) (out: t_FieldElement) -> true);
+    f_neg
+    =
+    fun (self: t_FieldElement) ->
+      Core_models.Ops.Arith.f_sub #t_FieldElement
+        #t_FieldElement
+        #FStar.Tactics.Typeclasses.solve
+        (Curve25519_dalek.Traits.f_identity #t_FieldElement #FStar.Tactics.Typeclasses.solve ()
+          <:
+          t_FieldElement)
+        self
+  }
+
+[@@ FStar.Tactics.Typeclasses.tcinstance]
+let impl_11: Core_models.Ops.Arith.t_Neg t_FieldElement =
+  {
+    f_Output = t_FieldElement;
+    f_neg_pre = (fun (self: t_FieldElement) -> true);
+    f_neg_post = (fun (self: t_FieldElement) (out: t_FieldElement) -> true);
+    f_neg
+    =
+    fun (self: t_FieldElement) ->
+      Core_models.Ops.Arith.f_neg #t_FieldElement #FStar.Tactics.Typeclasses.solve self
+  }
+
+/// Given `FieldElements` `u` and `v`, compute either `sqrt(u/v)`
+/// or `sqrt(i*u/v)` in constant time.
+/// This function always returns the nonnegative square root.
+/// # Return
+/// - `(Choice(1), +sqrt(u/v))  ` if `v` is nonzero and `u/v` is square;
+/// - `(Choice(1), zero)        ` if `u` is zero;
+/// - `(Choice(0), zero)        ` if `v` is zero and `u` is nonzero;
+/// - `(Choice(0), +sqrt(i*u/v))` if `u/v` is nonsquare (so `i*u/v` is square).
+let impl_6__sqrt_ratio_i (u v: t_FieldElement) : (Subtle.t_Choice & t_FieldElement) =
+  let v3:t_FieldElement =
+    Core_models.Ops.Arith.f_mul #t_FieldElement
+      #t_FieldElement
+      #FStar.Tactics.Typeclasses.solve
+      (impl_6__square v <: t_FieldElement)
+      v
+  in
+  let v7:t_FieldElement =
+    Core_models.Ops.Arith.f_mul #t_FieldElement
+      #t_FieldElement
+      #FStar.Tactics.Typeclasses.solve
+      (impl_6__square v3 <: t_FieldElement)
+      v
+  in
+  let r:t_FieldElement =
+    Core_models.Ops.Arith.f_mul #t_FieldElement
+      #t_FieldElement
+      #FStar.Tactics.Typeclasses.solve
+      (Core_models.Ops.Arith.f_mul #t_FieldElement
+          #t_FieldElement
+          #FStar.Tactics.Typeclasses.solve
+          u
+          v3
+        <:
+        t_FieldElement)
+      (impl_6__pow_p58 (Core_models.Ops.Arith.f_mul #t_FieldElement
+              #t_FieldElement
+              #FStar.Tactics.Typeclasses.solve
+              u
+              v7
+            <:
+            t_FieldElement)
+        <:
+        t_FieldElement)
+  in
+  let check:t_FieldElement =
+    Core_models.Ops.Arith.f_mul #t_FieldElement
+      #t_FieldElement
+      #FStar.Tactics.Typeclasses.solve
+      v
+      (impl_6__square r <: t_FieldElement)
+  in
+  let i:t_FieldElement = v_SQRT_M1 in
+  let correct_sign_sqrt:Subtle.t_Choice =
+    Subtle.f_ct_eq #t_FieldElement #FStar.Tactics.Typeclasses.solve check u
+  in
+  let flipped_sign_sqrt:Subtle.t_Choice =
+    Subtle.f_ct_eq #t_FieldElement
+      #FStar.Tactics.Typeclasses.solve
+      check
+      (Core_models.Ops.Arith.f_neg #t_FieldElement #FStar.Tactics.Typeclasses.solve u
+        <:
+        t_FieldElement)
+  in
+  let flipped_sign_sqrt_i:Subtle.t_Choice =
+    Subtle.f_ct_eq #t_FieldElement
+      #FStar.Tactics.Typeclasses.solve
+      check
+      (Core_models.Ops.Arith.f_mul #t_FieldElement
+          #t_FieldElement
+          #FStar.Tactics.Typeclasses.solve
+          (Core_models.Ops.Arith.f_neg #t_FieldElement #FStar.Tactics.Typeclasses.solve u
+            <:
+            t_FieldElement)
+          i
+        <:
+        t_FieldElement)
+  in
+  let r_prime:t_FieldElement =
+    Core_models.Ops.Arith.f_mul #t_FieldElement
+      #t_FieldElement
+      #FStar.Tactics.Typeclasses.solve
+      v_SQRT_M1
+      r
+  in
+  let r:t_FieldElement =
+    impl_6__conditional_assign r
+      r_prime
+      (Core_models.Ops.Bit.f_bitor #Subtle.t_Choice
+          #Subtle.t_Choice
+          #FStar.Tactics.Typeclasses.solve
+          flipped_sign_sqrt
+          flipped_sign_sqrt_i
+        <:
+        Subtle.t_Choice)
+  in
+  let r_is_negative:Subtle.t_Choice = impl_6__is_negative r in
+  let r:t_FieldElement = impl_6__conditional_negate r r_is_negative in
+  let was_nonzero_square:Subtle.t_Choice =
+    Core_models.Ops.Bit.f_bitor #Subtle.t_Choice
+      #Subtle.t_Choice
+      #FStar.Tactics.Typeclasses.solve
+      correct_sign_sqrt
+      flipped_sign_sqrt
+  in
+  was_nonzero_square, r <: (Subtle.t_Choice & t_FieldElement)
+
+/// Attempt to compute `sqrt(1/self)` in constant time.
+/// Convenience wrapper around `sqrt_ratio_i`.
+/// This function always returns the nonnegative square root.
+/// # Return
+/// - `(Choice(1), +sqrt(1/self))  ` if `self` is a nonzero square;
+/// - `(Choice(0), zero)           ` if `self` is zero;
+/// - `(Choice(0), +sqrt(i/self))  ` if `self` is a nonzero nonsquare;
+let impl_6__invsqrt (self: t_FieldElement) : (Subtle.t_Choice & t_FieldElement) =
+  impl_6__sqrt_ratio_i impl_6__ONE self
