proofs/fstar/extraction/Ristretto255.Bundle_decompress.fst
@@ -1,0 +1,336 @@
+module Ristretto255.Bundle_decompress
+#set-options "--fuel 0 --ifuel 1 --z3rlimit 15"
+open FStar.Mul
+open Core_models
+
+let _ =
+  (* This module has implicit dependencies, here we make them explicit. *)
+  (* The implicit dependencies arise from typeclasses instances. *)
+  let open Curve25519_dalek.Traits in
+  let open Ristretto255.Field in
+  let open Subtle in
+  ()
+
+/// A compressed Ristretto255 point.
+type t_CompressedRistretto =
+  | CompressedRistretto : t_Array u8 (mk_usize 32) -> t_CompressedRistretto
+
+let impl_6: Core_models.Clone.t_Clone t_CompressedRistretto =
+  { f_clone = (fun x -> x); f_clone_pre = (fun _ -> True); f_clone_post = (fun _ _ -> True) }
+
+[@@ FStar.Tactics.Typeclasses.tcinstance]
+assume
+val impl_5': Core_models.Marker.t_Copy t_CompressedRistretto
+
+unfold
+let impl_5 = impl_5'
+
+[@@ FStar.Tactics.Typeclasses.tcinstance]
+assume
+val impl_8': Core_models.Hash.t_Hash t_CompressedRistretto
+
+unfold
+let impl_8 = impl_8'
+
+[@@ FStar.Tactics.Typeclasses.tcinstance]
+let impl: Core_models.Cmp.t_PartialEq t_CompressedRistretto t_CompressedRistretto =
+  {
+    f_eq_pre = (fun (self: t_CompressedRistretto) (other: t_CompressedRistretto) -> true);
+    f_eq_post
+    =
+    (fun (self: t_CompressedRistretto) (other: t_CompressedRistretto) (out: bool) -> true);
+    f_eq
+    =
+    fun (self: t_CompressedRistretto) (other: t_CompressedRistretto) ->
+      Core_models.Convert.f_into #Subtle.t_Choice
+        #bool
+        #FStar.Tactics.Typeclasses.solve
+        (Subtle.f_ct_eq #(t_Slice u8)
+            #FStar.Tactics.Typeclasses.solve
+            (self._0 <: t_Slice u8)
+            (other._0 <: t_Slice u8)
+          <:
+          Subtle.t_Choice)
+  }
+
+[@@ FStar.Tactics.Typeclasses.tcinstance]
+assume
+val impl_7': Core_models.Cmp.t_Eq t_CompressedRistretto
+
+unfold
+let impl_7 = impl_7'
+
+/// Copy the bytes of this `CompressedRistretto`.
+let impl_9__to_bytes (self: t_CompressedRistretto) : t_Array u8 (mk_usize 32) = self._0
+
+/// View this `CompressedRistretto` as an array of bytes.
+let impl_9__as_bytes (self: t_CompressedRistretto) : t_Array u8 (mk_usize 32) = self._0
+
+[@@ FStar.Tactics.Typeclasses.tcinstance]
+let impl_1: Subtle.t_ConstantTimeEq t_CompressedRistretto =
+  {
+    f_ct_eq_pre = (fun (self: t_CompressedRistretto) (other: t_CompressedRistretto) -> true);
+    f_ct_eq_post
+    =
+    (fun (self: t_CompressedRistretto) (other: t_CompressedRistretto) (out: Subtle.t_Choice) -> true
+    );
+    f_ct_eq
+    =
+    fun (self: t_CompressedRistretto) (other: t_CompressedRistretto) ->
+      Subtle.f_ct_eq #(t_Slice u8)
+        #FStar.Tactics.Typeclasses.solve
+        (impl_9__as_bytes self <: t_Slice u8)
+        (impl_9__as_bytes other <: t_Slice u8)
+  }
+
+/// Construct a `CompressedRistretto` from a slice of bytes.
+/// # Errors
+/// Returns [`TryFromSliceError`] if the input `bytes` slice does not have
+/// a length of 32.
+let impl_9__from_slice (bytes: t_Slice u8)
+    : Prims.Pure
+      (Core_models.Result.t_Result t_CompressedRistretto Core_models.Array.t_TryFromSliceError)
+      (requires (Core_models.Slice.impl__len #u8 bytes <: usize) =. mk_usize 32)
+      (ensures
+        fun r ->
+          let r:Core_models.Result.t_Result t_CompressedRistretto
+            Core_models.Array.t_TryFromSliceError =
+            r
+          in
+          Core_models.Result.impl__is_ok #t_CompressedRistretto
+            #Core_models.Array.t_TryFromSliceError
+            r) =
+  Core_models.Result.impl__map #(t_Array u8 (mk_usize 32))
+    #Core_models.Array.t_TryFromSliceError
+    #t_CompressedRistretto
+    (Core_models.Convert.f_try_into #(t_Slice u8)
+        #(t_Array u8 (mk_usize 32))
+        #FStar.Tactics.Typeclasses.solve
+        bytes
+      <:
+      Core_models.Result.t_Result (t_Array u8 (mk_usize 32)) Core_models.Array.t_TryFromSliceError)
+    CompressedRistretto
+
+[@@ FStar.Tactics.Typeclasses.tcinstance]
+let impl_2: Curve25519_dalek.Traits.t_Identity t_CompressedRistretto =
+  {
+    f_identity_pre = (fun (_: Prims.unit) -> true);
+    f_identity_post = (fun (_: Prims.unit) (out: t_CompressedRistretto) -> true);
+    f_identity
+    =
+    fun (_: Prims.unit) ->
+      CompressedRistretto (Rust_primitives.Hax.repeat (mk_u8 0) (mk_usize 32))
+      <:
+      t_CompressedRistretto
+  }
+
+[@@ FStar.Tactics.Typeclasses.tcinstance]
+let impl_3: Core_models.Default.t_Default t_CompressedRistretto =
+  {
+    f_default_pre = (fun (_: Prims.unit) -> true);
+    f_default_post = (fun (_: Prims.unit) (out: t_CompressedRistretto) -> true);
+    f_default
+    =
+    fun (_: Prims.unit) ->
+      Curve25519_dalek.Traits.f_identity #t_CompressedRistretto #FStar.Tactics.Typeclasses.solve ()
+  }
+
+[@@ FStar.Tactics.Typeclasses.tcinstance]
+let impl_4: Core_models.Convert.t_TryFrom t_CompressedRistretto (t_Slice u8) =
+  {
+    f_Error = Core_models.Array.t_TryFromSliceError;
+    f_try_from_pre = (fun (slice: t_Slice u8) -> true);
+    f_try_from_post
+    =
+    (fun
+        (slice: t_Slice u8)
+        (out:
+          Core_models.Result.t_Result t_CompressedRistretto Core_models.Array.t_TryFromSliceError)
+        ->
+        true);
+    f_try_from = fun (slice: t_Slice u8) -> impl_9__from_slice slice
+  }
+
+type t_EdwardsPoint = {
+  f_X:Ristretto255.Field.t_FieldElement;
+  f_Y:Ristretto255.Field.t_FieldElement;
+  f_Z:Ristretto255.Field.t_FieldElement;
+  f_T:Ristretto255.Field.t_FieldElement
+}
+
+type t_RistrettoPoint = | RistrettoPoint : t_EdwardsPoint -> t_RistrettoPoint
+
+let step_1_ (repr: t_CompressedRistretto)
+    : (Subtle.t_Choice & Subtle.t_Choice & Ristretto255.Field.t_FieldElement) =
+  let s:Ristretto255.Field.t_FieldElement =
+    Ristretto255.Field.impl_FieldElement__from_bytes (impl_9__as_bytes repr
+        <:
+        t_Array u8 (mk_usize 32))
+  in
+  let s_bytes_check:t_Array u8 (mk_usize 32) = Ristretto255.Field.impl_FieldElement__to_bytes s in
+  let s_encoding_is_canonical:Subtle.t_Choice =
+    Subtle.f_ct_eq #(t_Slice u8)
+      #FStar.Tactics.Typeclasses.solve
+      (s_bytes_check.[ Core_models.Ops.Range.RangeFull <: Core_models.Ops.Range.t_RangeFull ]
+        <:
+        t_Slice u8)
+      (impl_9__as_bytes repr <: t_Slice u8)
+  in
+  let s_is_negative:Subtle.t_Choice = Ristretto255.Field.impl_FieldElement__is_negative s in
+  s_encoding_is_canonical, s_is_negative, s
+  <:
+  (Subtle.t_Choice & Subtle.t_Choice & Ristretto255.Field.t_FieldElement)
+
+let step_2_ (s: Ristretto255.Field.t_FieldElement)
+    : (Subtle.t_Choice & Subtle.t_Choice & Subtle.t_Choice & t_RistrettoPoint) =
+  let one:Ristretto255.Field.t_FieldElement = Ristretto255.Field.impl_FieldElement__ONE in
+  let ss:Ristretto255.Field.t_FieldElement = Ristretto255.Field.impl_FieldElement__square s in
+  let u1:Ristretto255.Field.t_FieldElement =
+    Core_models.Ops.Arith.f_sub #Ristretto255.Field.t_FieldElement
+      #Ristretto255.Field.t_FieldElement
+      #FStar.Tactics.Typeclasses.solve
+      one
+      ss
+  in
+  let u2:Ristretto255.Field.t_FieldElement =
+    Core_models.Ops.Arith.f_add #Ristretto255.Field.t_FieldElement
+      #Ristretto255.Field.t_FieldElement
+      #FStar.Tactics.Typeclasses.solve
+      one
+      ss
+  in
+  let u2_sqr:Ristretto255.Field.t_FieldElement = Ristretto255.Field.impl_FieldElement__square u2 in
+  let v:Ristretto255.Field.t_FieldElement =
+    Core_models.Ops.Arith.f_sub #Ristretto255.Field.t_FieldElement
+      #Ristretto255.Field.t_FieldElement
+      #FStar.Tactics.Typeclasses.solve
+      (Core_models.Ops.Arith.f_mul #Ristretto255.Field.t_FieldElement
+          #Ristretto255.Field.t_FieldElement
+          #FStar.Tactics.Typeclasses.solve
+          (Core_models.Ops.Arith.f_neg #Ristretto255.Field.t_FieldElement
+              #FStar.Tactics.Typeclasses.solve
+              Ristretto255.Constants.v_EDWARDS_D
+            <:
+            Ristretto255.Field.t_FieldElement)
+          (Ristretto255.Field.impl_FieldElement__square u1 <: Ristretto255.Field.t_FieldElement)
+        <:
+        Ristretto255.Field.t_FieldElement)
+      u2_sqr
+  in
+  let (ok: Subtle.t_Choice), (v_I: Ristretto255.Field.t_FieldElement) =
+    Ristretto255.Field.impl_FieldElement__invsqrt (Core_models.Ops.Arith.f_mul #Ristretto255.Field.t_FieldElement
+          #Ristretto255.Field.t_FieldElement
+          #FStar.Tactics.Typeclasses.solve
+          v
+          u2_sqr
+        <:
+        Ristretto255.Field.t_FieldElement)
+  in
+  let v_Dx:Ristretto255.Field.t_FieldElement =
+    Core_models.Ops.Arith.f_mul #Ristretto255.Field.t_FieldElement
+      #Ristretto255.Field.t_FieldElement
+      #FStar.Tactics.Typeclasses.solve
+      v_I
+      u2
+  in
+  let v_Dy:Ristretto255.Field.t_FieldElement =
+    Core_models.Ops.Arith.f_mul #Ristretto255.Field.t_FieldElement
+      #Ristretto255.Field.t_FieldElement
+      #FStar.Tactics.Typeclasses.solve
+      v_I
+      (Core_models.Ops.Arith.f_mul #Ristretto255.Field.t_FieldElement
+          #Ristretto255.Field.t_FieldElement
+          #FStar.Tactics.Typeclasses.solve
+          v_Dx
+          v
+        <:
+        Ristretto255.Field.t_FieldElement)
+  in
+  let x:Ristretto255.Field.t_FieldElement =
+    Core_models.Ops.Arith.f_mul #Ristretto255.Field.t_FieldElement
+      #Ristretto255.Field.t_FieldElement
+      #FStar.Tactics.Typeclasses.solve
+      (Core_models.Ops.Arith.f_add #Ristretto255.Field.t_FieldElement
+          #Ristretto255.Field.t_FieldElement
+          #FStar.Tactics.Typeclasses.solve
+          s
+          s
+        <:
+        Ristretto255.Field.t_FieldElement)
+      v_Dx
+  in
+  let x_neg:Subtle.t_Choice = Ristretto255.Field.impl_FieldElement__is_negative x in
+  let x:Ristretto255.Field.t_FieldElement =
+    Ristretto255.Field.impl_FieldElement__conditional_negate x x_neg
+  in
+  let y:Ristretto255.Field.t_FieldElement =
+    Core_models.Ops.Arith.f_mul #Ristretto255.Field.t_FieldElement
+      #Ristretto255.Field.t_FieldElement
+      #FStar.Tactics.Typeclasses.solve
+      u1
+      v_Dy
+  in
+  let t:Ristretto255.Field.t_FieldElement =
+    Core_models.Ops.Arith.f_mul #Ristretto255.Field.t_FieldElement
+      #Ristretto255.Field.t_FieldElement
+      #FStar.Tactics.Typeclasses.solve
+      x
+      y
+  in
+  ok,
+  Ristretto255.Field.impl_FieldElement__is_negative t,
+  Ristretto255.Field.impl_FieldElement__is_zero y,
+  (RistrettoPoint ({ f_X = x; f_Y = y; f_Z = one; f_T = t } <: t_EdwardsPoint) <: t_RistrettoPoint)
+  <:
+  (Subtle.t_Choice & Subtle.t_Choice & Subtle.t_Choice & t_RistrettoPoint)
+
+/// Attempt to decompress to an `RistrettoPoint`.
+/// # Return
+/// - `Some(RistrettoPoint)` if `self` was the canonical encoding of a point;
+/// - `None` if `self` was not the canonical encoding of a point.
+let impl_9__decompress (self: t_CompressedRistretto) : Core_models.Option.t_Option t_RistrettoPoint =
+  let
+  (s_encoding_is_canonical: Subtle.t_Choice),
+  (s_is_negative: Subtle.t_Choice),
+  (s: Ristretto255.Field.t_FieldElement) =
+    step_1_ self
+  in
+  if
+    Core_models.Convert.f_into #Subtle.t_Choice
+      #bool
+      #FStar.Tactics.Typeclasses.solve
+      (Core_models.Ops.Bit.f_bitor #Subtle.t_Choice
+          #Subtle.t_Choice
+          #FStar.Tactics.Typeclasses.solve
+          (~.s_encoding_is_canonical <: Subtle.t_Choice)
+          s_is_negative
+        <:
+        Subtle.t_Choice)
+  then Core_models.Option.Option_None <: Core_models.Option.t_Option t_RistrettoPoint
+  else
+    let
+    (ok: Subtle.t_Choice),
+    (tt_is_negative: Subtle.t_Choice),
+    (y_is_zero: Subtle.t_Choice),
+    (res: t_RistrettoPoint) =
+      step_2_ s
+    in
+    if
+      Core_models.Convert.f_into #Subtle.t_Choice
+        #bool
+        #FStar.Tactics.Typeclasses.solve
+        (Core_models.Ops.Bit.f_bitor #Subtle.t_Choice
+            #Subtle.t_Choice
+            #FStar.Tactics.Typeclasses.solve
+            (Core_models.Ops.Bit.f_bitor #Subtle.t_Choice
+                #Subtle.t_Choice
+                #FStar.Tactics.Typeclasses.solve
+                (~.ok <: Subtle.t_Choice)
+                tt_is_negative
+              <:
+              Subtle.t_Choice)
+            y_is_zero
+          <:
+          Subtle.t_Choice)
+    then Core_models.Option.Option_None <: Core_models.Option.t_Option t_RistrettoPoint
+    else Core_models.Option.Option_Some res <: Core_models.Option.t_Option t_RistrettoPoint
