proofs/fstar/extraction/Ristretto255.Field.fst
@@ -1,0 +1,66 @@
+module Ristretto255.Field
+#set-options "--fuel 0 --ifuel 1 --z3rlimit 15"
+open FStar.Mul
+open Core_models
+
+include Ristretto255.Bundle {t_FieldElement as t_FieldElement}
+
+include Ristretto255.Bundle {FieldElement as FieldElement}
+
+include Ristretto255.Bundle {impl_12 as impl_12}
+
+include Ristretto255.Bundle {impl_13 as impl_13}
+
+include Ristretto255.Bundle {impl_14 as impl_14}
+
+include Ristretto255.Bundle {impl_15 as impl_15}
+
+include Ristretto255.Bundle {impl_16 as impl_16}
+
+include Ristretto255.Bundle {impl_17 as impl_17}
+
+include Ristretto255.Bundle {impl as impl}
+
+include Ristretto255.Bundle {impl_1 as impl_1}
+
+include Ristretto255.Bundle {impl_2 as impl_2}
+
+include Ristretto255.Bundle {impl_3 as impl_3}
+
+include Ristretto255.Bundle {impl_4 as impl_4}
+
+include Ristretto255.Bundle {impl_5 as impl_5}
+
+include Ristretto255.Bundle {impl_6__ONE as impl_FieldElement__ONE}
+
+include Ristretto255.Bundle {impl_6__from_bytes as impl_FieldElement__from_bytes}
+
+include Ristretto255.Bundle {impl_6__to_bytes as impl_FieldElement__to_bytes}
+
+include Ristretto255.Bundle {impl_6__square as impl_FieldElement__square}
+
+include Ristretto255.Bundle {impl_6__is_negative as impl_FieldElement__is_negative}
+
+include Ristretto255.Bundle {impl_6__is_zero as impl_FieldElement__is_zero}
+
+include Ristretto255.Bundle {impl_6__conditional_negate as impl_FieldElement__conditional_negate}
+
+include Ristretto255.Bundle {impl_6__conditional_assign as impl_FieldElement__conditional_assign}
+
+include Ristretto255.Bundle {impl_6__invsqrt as impl_FieldElement__invsqrt}
+
+include Ristretto255.Bundle {impl_6__sqrt_ratio_i as impl_FieldElement__sqrt_ratio_i}
+
+include Ristretto255.Bundle {impl_6__pow_p58 as impl_FieldElement__pow_p58}
+
+include Ristretto255.Bundle {impl_6__from_bytes__load8_at as impl_FieldElement__from_bytes__load8_at}
+
+include Ristretto255.Bundle {impl_7 as impl_7}
+
+include Ristretto255.Bundle {impl_8 as impl_8}
+
+include Ristretto255.Bundle {impl_9 as impl_9}
+
+include Ristretto255.Bundle {impl_10 as impl_10}
+
+include Ristretto255.Bundle {impl_11 as impl_11}
